backend/LTL.v
@@ -216,10 +216,10 @@ Inductive state : Type :=
              (cp: compartment),       (**r compartment we're returning from *)
       state.
 
-Definition call_comp (stack: list stackframe) : option compartment :=
+Definition call_comp (stack: list stackframe) : compartment :=
   match stack with
-  | nil => None
-  | Stackframe f _ _ _ _ :: _ => Some (comp_of f)
+  | nil => bottom
+  | Stackframe f _ _ _ _ :: _ =>  comp_of f
   end.
 
 Section RELSEM.
@@ -307,7 +307,7 @@ Inductive step: state -> trace -> state -> Prop :=
         E0 (Block s f sp bb rs' m)
   | exec_Lload: forall s f sp chunk addr args dst bb rs m a v rs',
       eval_addressing ge sp addr (reglist rs args) = Some a ->
-      Mem.loadv chunk m a (Some (comp_of f)) = Some v ->
+      Mem.loadv chunk m a (comp_of f) = Some v ->
       rs' = Locmap.set (R dst) v (undef_regs (destroyed_by_load chunk addr) rs) ->
       step (Block s f sp (Lload chunk addr args dst :: bb) rs m)
         E0 (Block s f sp bb rs' m)
@@ -351,9 +351,9 @@ Inductive step: state -> trace -> state -> Prop :=
         E0 (Callstate s fd sig rs' m')
   | exec_Lbuiltin: forall s f sp ef args res bb rs m vargs t vres rs' m',
       eval_builtin_args ge rs sp m args vargs ->
-      external_call ef ge vargs m t vres m' ->
+      external_call ef ge (comp_of f) vargs m t vres m' ->
       rs' = Locmap.setres res vres (undef_regs (destroyed_by_builtin ef) rs) ->
-      forall ALLOWED: comp_of f = comp_of ef,
+      (* forall ALLOWED: comp_of f = comp_of ef, *)
       step (Block s f sp (Lbuiltin ef args res :: bb) rs m)
          t (Block s f sp bb rs' m')
   | exec_Lbranch: forall s f sp pc bb rs m,
@@ -388,10 +388,10 @@ Inductive step: state -> trace -> state -> Prop :=
         E0 (State s f (Vptr sp Ptrofs.zero) f.(fn_entrypoint) rs' m')
   | exec_function_external: forall s ef t args res rs m rs' sig m',
       args = map (fun p => Locmap.getpair p rs) (loc_arguments (ef_sig ef)) ->
-      external_call ef ge args m t res m' ->
+      external_call ef ge (call_comp s) args m t res m' ->
       rs' = Locmap.setpair (loc_result (ef_sig ef)) res (undef_caller_save_regs rs) ->
       step (Callstate s (External ef) sig rs m)
-         t (Returnstate s rs' m' (comp_of ef))
+         t (Returnstate s rs' m' (call_comp s))
   | exec_return: forall f sp rs1 bb s rs m cp sig t,
       forall (NO_CROSS_PTR:
           Genv.type_of_call (comp_of f) cp = Genv.CrossCompartmentCall ->
